Added text to Q4

src/LAB3/Q4.dfy
@@ -1,13 +1,117 @@
 
     /* Question 1 Task 1:
-     multi-line comment
-     span accross multiple
-     lines */
+     function fact(n : nat) : nat
+     {
+       if (n <= 1) then 1 else n * fact(n-1)
+     }
+
+     method ComputeFact(n : nat) returns (res : nat)
+       requires n > 0;
+       ensures res == fact(n);
+      {
+       res := 1;
+       var i := 2;
+       while (i <= n)
+       decreases n - i + 1;
+       invariant i <= n+1;
+       invariant res == fact(i-1);
+       {
+         res := res * i;
+         i := i + 1;
+       }
+      }
+*/
 
      /* Question 1 Task 2:
-     multi-line comment
-     span accross multiple
-     lines */
+
+//Total correctness:
+wp(while B I D S, R) =
+//1   I
+//2   && (B && I ==> wp(S,I))
+//3   && (!B && I ==> R)
+
+//4   && (I ==> D >= 0)
+//5   && (B && I ==>
+       wp(tmp := D ; S, tmp > D))
+
+
+//1	 (i <= n+1 ^ res == fact(i-1))
+//2	^( (i <= n) ^ (i <= n+1 ^ res == fact(i-1)) ⇒
+        wp(res := res * i; i := i + 1, (i <= n+1 ^ res == fact(i-1))) )
+//3	^( (i > n) ^ (i <= n+1 ^ res == fact(i-1))==> res == fact(n)) )
+
+//4	^( (i <= n+1 ^ res == fact(i-1)) ⇒ n-i+1 >= 0 )
+//5	^( (i <= n) ^ (i <= n+1 ^ res == fact(i-1)) ⇒
+        wp(tmp := n-i+1; res := res * i; i := i + 1, (tmp > n-i+1)) )
+
+//Start by proving 2
+(i <= n) ^ (i <= n+1 ^ res == fact(i-1)) ⇒
+        wp(res := res * i; i := i + 1, (i <= n+1 ^ res == fact(i-1)))
+//Solve the wp
+//Sequential rule
+wp(res := res * i, wp(i := i + 1, (i <= n+1 ^ res == fact(i-1))))
+//Assignment rule
+= wp(res := res * i, (i+1 <= n+1 ^ res == fact(i)))
+//Assignment rule
+= i+1 <= n+1 ^ res * i == fact(i)
+//Simplify
+= i <= n ^ res * i == fact(i)
+
+(i <= n) ^ (i <= n+1 ^ res == fact(i-1)) ⇒
+(i <= n) ^ (res * i == fact(i))
+//Simplify
+(res == fact(i-1)) ⇒
+(res * i == fact(i))
+//Simplify
+fact(i-1)*i == fact(i) (true per definition of factorial)
+
+//2 is true.
+
+//Continue by proving 3
+(i > n) ^ (i <= n+1 ^ res == fact(i-1))==> res == fact(n))
+(i == (n+1)) ^ (res == fact(i-1))==> res == fact(n)
+res == fact((n+1)-1) ⇒ res == fact(n)
+res == fact(n) ⇒ res == fact(n) (trivially true)
+
+//3 is true
+
+//Continue by proving 4
+(i <= n+1 ^ res == fact(i-1)) ⇒ n-i >= 0
+i <= n+1 ⇒ n-i+1 >= 0
+i <= n+1 ⇒ (n+1)-i >= 0 (if i==(n+1), (n+1)-i==0, else (n+1)-i>0
+i <= n+1 ⇒ n-i+1 >= 0 (true)
+
+//4 is true
+
+
+//Continue by proving 5
+(i <= n) ^ (i <= n+1 ^ res == fact(i-1)) ⇒
+    wp(tmp := n-i+1; res := res * i; i := i + 1, (tmp > n-i+1))
+
+//Solve the wp
+//Sequential rule
+wp(tmp := n-i+1; res := res * i, wp(i := i + 1, (tmp > n-i+1)))
+//Assignment rule
+wp(tmp := n-i+1; res := res * i, (tmp > n-(i + 1)+1))
+//Sequential rule
+wp(tmp := n-i+1, wp(res := res * i, (tmp > n-(i + 1)+1)))
+//Assignment rule
+wp(tmp := n-i+1,(tmp > n-(i + 1)+1))
+//Assignment rule
+n-i+1 > n-(i + 1)+1
+//Simplify
+n-i+1 > n-i (trivially true)
+
+//5 is true
+
+//All that is left is 1 which is the invariant
+(i <= n+1 ^ res == fact(i-1))
+
+//This means that if the invariant is true when entering the loop then the loop is correct. The loop is verified to be correct.
+
+
+
+      */
 
 
 
